Definition of Refinement
1. change state simulation to state relation
2. try to define simulation in PiCore_Sim

Refinement.thy
@@ -17,16 +17,238 @@ locale SM_Refine =
   and obs\<^sub>a :: "'s\<^sub>a \<Rightarrow> 'd \<Rightarrow> 'o\<^sub>a" (infixl "\<guillemotright>\<^sub>a"  55)
   and vpeq\<^sub>a :: "'s\<^sub>a \<Rightarrow> 'd \<Rightarrow> 's\<^sub>a \<Rightarrow> bool" ("(_ \<sim>\<^sub>a_\<sim>\<^sub>a _)" [70,69,70] 60)
   and interference\<^sub>a :: "'d \<Rightarrow> 'd \<Rightarrow> bool" ("(_ \<leadsto>\<^sub>a _)" [70,71] 60) + 
-fixes sim_s :: "'s\<^sub>c \<Rightarrow> 's\<^sub>a"
+fixes sim_s :: "'s\<^sub>c \<Rightarrow> 's\<^sub>a \<Rightarrow> bool" ("(_ \<sim> _)" [70,70] 60)
   and sim_a :: "'a\<^sub>c \<Rightarrow> 'a\<^sub>a option"
 assumes
-  init_sim : "sim_s s0\<^sub>c = s0\<^sub>a" and
-  action_refine : "sim_a a\<^sub>c = Some a\<^sub>a \<longrightarrow> (s\<^sub>c, t\<^sub>c) \<in> step\<^sub>c a\<^sub>c \<longrightarrow> (sim_s s\<^sub>c, sim_s t\<^sub>c) \<in> step\<^sub>a a\<^sub>a" and
-  none_refine : "sim_a a\<^sub>c = None \<longrightarrow> (s\<^sub>c, t\<^sub>c) \<in> step\<^sub>c a\<^sub>c \<longrightarrow> sim_s s\<^sub>c = sim_s t\<^sub>c" and
+  init_sim : " s0\<^sub>c \<sim> s0\<^sub>a" and
+  action_refine : "\<lbrakk>sim_a a\<^sub>c = Some a\<^sub>a; SM_IFS\<^sub>c.reachable0 s\<^sub>c; s\<^sub>c \<sim> s\<^sub>a; (s\<^sub>c, t\<^sub>c) \<in> step\<^sub>c a\<^sub>c\<rbrakk> 
+            \<Longrightarrow> \<exists>t\<^sub>a. t\<^sub>c \<sim> t\<^sub>a \<and> (s\<^sub>a, t\<^sub>a) \<in> step\<^sub>a a\<^sub>a" and
+  none_refine : "\<lbrakk>sim_a a\<^sub>c = None; SM_IFS\<^sub>c.reachable0 s\<^sub>c; s\<^sub>c \<sim> s\<^sub>a; (s\<^sub>c, t\<^sub>c) \<in> step\<^sub>c a\<^sub>c\<rbrakk> \<Longrightarrow> t\<^sub>c \<sim> s\<^sub>a" and
   intefere_same : "interference\<^sub>c = interference\<^sub>a" and 
   dom_refine : "sim_a a\<^sub>c = Some a\<^sub>a \<longrightarrow> domain\<^sub>c a\<^sub>c = domain\<^sub>a a\<^sub>a" and 
+  sim_ifs : " \<lbrakk>s\<^sub>c \<sim> s\<^sub>a; t\<^sub>c \<sim> t\<^sub>a\<rbrakk> \<Longrightarrow> s\<^sub>a \<sim>\<^sub>a d \<sim>\<^sub>a t\<^sub>a = s\<^sub>c \<sim>\<^sub>c d \<sim>\<^sub>c t\<^sub>c" 
+begin 
+
+abbreviation reachable0\<^sub>c :: "'s\<^sub>c \<Rightarrow> bool"
+  where "reachable0\<^sub>c \<equiv> SM_IFS\<^sub>c.reachable0"
+
+abbreviation reachable0\<^sub>a :: "'s\<^sub>a \<Rightarrow> bool"
+  where "reachable0\<^sub>a \<equiv> SM_IFS\<^sub>a.reachable0"
+
+abbreviation run\<^sub>c :: " 'a\<^sub>c list \<Rightarrow> ('s\<^sub>c \<times> 's\<^sub>c) set"
+  where "run\<^sub>c \<equiv> SM_IFS\<^sub>c.run"
+
+abbreviation execute\<^sub>c :: "'a\<^sub>c list \<Rightarrow> 's\<^sub>c \<Rightarrow> 's\<^sub>c set"
+  where "execute\<^sub>c \<equiv> SM_IFS\<^sub>c.execute"
+
+lemma reachR_reach1: "\<forall>s\<^sub>c as\<^sub>c t\<^sub>c s\<^sub>a. reachable0\<^sub>a s\<^sub>a \<and> reachable0\<^sub>c s\<^sub>c \<and> s\<^sub>c \<sim> s\<^sub>a \<and> t\<^sub>c \<in> execute\<^sub>c as\<^sub>c s\<^sub>c
+                        \<longrightarrow> (\<exists>t\<^sub>a. t\<^sub>c \<sim> t\<^sub>a \<and> reachable0\<^sub>a t\<^sub>a)"
+proof -
+  {
+    fix as\<^sub>c
+    have "\<forall>s\<^sub>c t\<^sub>c s\<^sub>a. reachable0\<^sub>a s\<^sub>a \<and> reachable0\<^sub>c s\<^sub>c \<and> s\<^sub>c \<sim> s\<^sub>a \<and> t\<^sub>c \<in> execute\<^sub>c as\<^sub>c s\<^sub>c
+                        \<longrightarrow> (\<exists>t\<^sub>a. t\<^sub>c \<sim> t\<^sub>a \<and> reachable0\<^sub>a t\<^sub>a)"
+    proof(induct as\<^sub>c)
+      case Nil show ?case 
+        using SM_IFS\<^sub>c.execute_def by auto
+    next
+      case (Cons b\<^sub>c bs\<^sub>c)
+      assume a0: "\<forall>s\<^sub>c t\<^sub>c s\<^sub>a. reachable0\<^sub>a s\<^sub>a \<and> reachable0\<^sub>c s\<^sub>c \<and> s\<^sub>c \<sim> s\<^sub>a \<and> t\<^sub>c \<in> execute\<^sub>c bs\<^sub>c s\<^sub>c 
+                  \<longrightarrow> (\<exists>t\<^sub>a. t\<^sub>c \<sim> t\<^sub>a \<and> reachable0\<^sub>a t\<^sub>a)"
+      show ?case
+      proof -
+        {
+          fix s\<^sub>c t\<^sub>c s\<^sub>a
+          assume b0: "reachable0\<^sub>a s\<^sub>a \<and> reachable0\<^sub>c s\<^sub>c \<and> s\<^sub>c \<sim> s\<^sub>a \<and> t\<^sub>c \<in> execute\<^sub>c (b\<^sub>c # bs\<^sub>c) s\<^sub>c"
+          have b1: "\<forall>s\<^sub>c'. (s\<^sub>c, s\<^sub>c') \<in> step\<^sub>c b\<^sub>c \<longrightarrow> (\<exists>s\<^sub>a'. s\<^sub>c' \<sim> s\<^sub>a' \<and> reachable0\<^sub>a s\<^sub>a')"
+          proof-
+            {
+              fix s\<^sub>c'
+              assume c0: "(s\<^sub>c, s\<^sub>c') \<in> step\<^sub>c b\<^sub>c"
+              have "\<exists>s\<^sub>a'. s\<^sub>c' \<sim> s\<^sub>a' \<and> reachable0\<^sub>a s\<^sub>a'"
+              proof(cases "sim_a b\<^sub>c = None")
+                assume d0: "sim_a b\<^sub>c = None"
+                with b0 c0 have "s\<^sub>c' \<sim> s\<^sub>a"
+                  using none_refine by blast
+                then show ?thesis
+                  using b0 by blast
+              next
+                assume e0: "sim_a b\<^sub>c \<noteq> None"
+                then have "\<exists>b\<^sub>a. sim_a b\<^sub>c = Some b\<^sub>a" by simp
+                then obtain b\<^sub>a where e1: "sim_a b\<^sub>c = Some b\<^sub>a" by auto
+                then have "\<exists>s\<^sub>a'. s\<^sub>c' \<sim> s\<^sub>a' \<and> (s\<^sub>a, s\<^sub>a') \<in> step\<^sub>a b\<^sub>a"
+                  using action_refine b0 c0 by blast
+                then obtain s\<^sub>a' where e2: "s\<^sub>c' \<sim> s\<^sub>a' \<and> (s\<^sub>a, s\<^sub>a') \<in> step\<^sub>a b\<^sub>a" by auto
+                then show ?thesis 
+                  using SM_IFS\<^sub>a.reachableStep b0 by blast
+              qed
+            }          
+            then show ?thesis by auto
+          qed
+          from b0 have "\<exists>s\<^sub>c'. (s\<^sub>c, s\<^sub>c') \<in> step\<^sub>c b\<^sub>c \<and> (s\<^sub>c', t\<^sub>c) \<in> run\<^sub>c bs\<^sub>c"
+            using SM_IFS\<^sub>c.execute_def by auto
+          then obtain s\<^sub>c' where b2: "(s\<^sub>c, s\<^sub>c') \<in> step\<^sub>c b\<^sub>c \<and> (s\<^sub>c', t\<^sub>c) \<in> run\<^sub>c bs\<^sub>c" by auto
+          with b1 have "\<exists>s\<^sub>a'. s\<^sub>c' \<sim> s\<^sub>a' \<and> reachable0\<^sub>a s\<^sub>a'" by blast
+          then obtain s\<^sub>a' where b3: " s\<^sub>c' \<sim> s\<^sub>a' \<and> reachable0\<^sub>a s\<^sub>a'" by auto
+          have b4: "reachable0\<^sub>c s\<^sub>c'"
+            using SM_IFS\<^sub>c.reachableStep b0 b2 by blast
+          with a0 b2 b3 have "\<exists>t\<^sub>a. t\<^sub>c \<sim> t\<^sub>a \<and> reachable0\<^sub>a t\<^sub>a"
+            using SM_IFS\<^sub>c.execute_def by auto
+        }
+        then show ?thesis by auto
+      qed
+    qed
+  }
+  then show ?thesis by auto
+qed
+
+lemma reachR_reach: "reachable0\<^sub>c s\<^sub>c \<Longrightarrow> \<exists>s\<^sub>a. s\<^sub>c \<sim> s\<^sub>a \<and> reachable0\<^sub>a s\<^sub>a"
+  by (metis Image_singleton_iff SM_IFS.execute_def SM_IFS\<^sub>a.reachableC0 SM_IFS\<^sub>c.SM_IFS_axioms 
+     SM_IFS\<^sub>c.reachable0_def SM_IFS\<^sub>c.reachableC0 SM_IFS\<^sub>c.reachable_def init_sim reachR_reach1)
+
+theorem abs_lr_imp : "SM_IFS\<^sub>a.local_respect \<Longrightarrow> SM_IFS\<^sub>c.local_respect"
+proof-
+  assume a0: "SM_IFS\<^sub>a.local_respect"
+  then have a1: "\<forall>aa d sa sa'. reachable0\<^sub>a sa \<longrightarrow> \<not> domain\<^sub>a aa \<leadsto>\<^sub>a d 
+                 \<and> (sa, sa') \<in> step\<^sub>a aa \<longrightarrow> (sa \<sim>\<^sub>a d \<sim>\<^sub>a sa')"
+    by (simp add: SM_IFS\<^sub>a.local_respect_def)
+  have "\<forall>ac d sc sc'. reachable0\<^sub>c sc \<longrightarrow> \<not> domain\<^sub>c ac \<leadsto>\<^sub>a d \<and> (sc, sc') \<in> step\<^sub>c ac 
+                      \<longrightarrow> (sc \<sim>\<^sub>c d \<sim>\<^sub>c sc')"
+  proof-
+    {
+      fix ac d sc sc'
+      assume b0: "reachable0\<^sub>c sc"
+        and  b1: "\<not> domain\<^sub>c ac \<leadsto>\<^sub>a d"
+        and  b2: "(sc, sc') \<in> step\<^sub>c ac "
+      from b0 have  "\<exists>sa. sc \<sim> sa \<and> reachable0\<^sub>a sa" by (simp add: reachR_reach)
+      then obtain sa where b3: "sc \<sim> sa \<and> reachable0\<^sub>a sa" by auto
+      have "sc \<sim>\<^sub>c d \<sim>\<^sub>c sc'"
+      proof(cases "sim_a ac = None")
+        assume c0: "sim_a ac = None"
+        with b0 b2 b3 have "sc' \<sim> sa"by (simp add: none_refine)
+        then show ?thesis
+          by (meson SM_IFS\<^sub>a.vpeq_reflexive SM_Refine.sim_ifs SM_Refine_axioms b3)
+      next
+        assume d0: "\<not> sim_a ac = None"
+        then have  "\<exists>aa. sim_a ac = Some aa" by auto
+        then obtain aa where d1: "sim_a ac = Some aa" by force
+        then have d01: "domain\<^sub>c ac = domain\<^sub>a aa"
+          by (simp add: dom_refine)
+        with b1 have d2 :"\<not> domain\<^sub>c ac \<leadsto>\<^sub>a d"
+          by (simp add: intefere_same)
+        from b0 b2 b3 have "\<exists>sa'. sc' \<sim> sa' \<and> (sa, sa') \<in> step\<^sub>a aa"
+          using SM_Refine.action_refine SM_Refine_axioms d1 by fastforce
+        then obtain sa' where d3: "sc' \<sim> sa' \<and> (sa, sa') \<in> step\<^sub>a aa" by auto
+        with a1 d2 d3 have " sa \<sim>\<^sub>a d \<sim>\<^sub>a sa'"
+          using b3 d01 by auto
+        then show ?thesis
+          using b3 d3 sim_ifs by blast
+      qed
+    }
+    then show ?thesis by auto
+  qed
+  then show ?thesis 
+    using SM_IFS\<^sub>c.local_respect_def intefere_same by blast
+qed
+
+
+theorem abs_wsc_imp : "SM_IFS\<^sub>a.weak_step_consistent \<Longrightarrow> SM_IFS\<^sub>c.weak_step_consistent"
+proof-
+  assume a0: "SM_IFS\<^sub>a.weak_step_consistent"
+  then have a1: "\<forall>aa d sa ta. reachable0\<^sub>a sa \<and> reachable0\<^sub>a ta \<longrightarrow> (sa \<sim>\<^sub>a d \<sim>\<^sub>a ta) \<and> 
+                 (domain\<^sub>a aa \<leadsto>\<^sub>a d \<longrightarrow> sa \<sim>\<^sub>a domain\<^sub>a aa \<sim>\<^sub>a ta) 
+                 \<longrightarrow> (\<forall>sa' ta'. (sa, sa') \<in> step\<^sub>a aa \<and> (ta, ta') \<in> step\<^sub>a aa \<longrightarrow> sa' \<sim>\<^sub>a d \<sim>\<^sub>a ta')"
+    using SM_IFS\<^sub>a.weak_step_consistent_def by blast
+  have "\<forall>ac d sc tc. reachable0\<^sub>c sc \<and> reachable0\<^sub>c tc \<longrightarrow> (sc \<sim>\<^sub>c d \<sim>\<^sub>c tc) \<and> 
+                 (domain\<^sub>c ac \<leadsto>\<^sub>c d \<longrightarrow> sc \<sim>\<^sub>c domain\<^sub>c ac \<sim>\<^sub>c tc) 
+                 \<longrightarrow> (\<forall>sc' tc'. (sc, sc') \<in> step\<^sub>c ac \<and> (tc, tc') \<in> step\<^sub>c ac \<longrightarrow> sc' \<sim>\<^sub>c d \<sim>\<^sub>c tc')"
+  proof-
+    {
+      fix ac d sc tc
+      assume b0: "reachable0\<^sub>c sc"
+        and  b1: "reachable0\<^sub>c tc"
+        and  b2: "sc \<sim>\<^sub>c d \<sim>\<^sub>c tc"
+        and  b3: "domain\<^sub>c ac \<leadsto>\<^sub>c d \<longrightarrow> sc \<sim>\<^sub>c domain\<^sub>c ac \<sim>\<^sub>c tc"
+      from b0 have "\<exists>sa. sc \<sim> sa \<and> reachable0\<^sub>a sa"
+        using reachR_reach by blast
+      then obtain sa where b4: "sc \<sim> sa \<and> reachable0\<^sub>a sa" by auto
+      from b1 have "\<exists>ta. tc \<sim> ta \<and> reachable0\<^sub>a ta"
+        using reachR_reach by blast
+      then obtain ta where b5: "tc \<sim> ta \<and> reachable0\<^sub>a ta" by auto
+      have "\<forall>sc' tc'. (sc, sc') \<in> step\<^sub>c ac \<and> (tc, tc') \<in> step\<^sub>c ac \<longrightarrow> sc' \<sim>\<^sub>c d \<sim>\<^sub>c tc'"
+      proof-
+        {
+          fix sc' tc'
+          assume c0: "(sc,sc') \<in> step\<^sub>c ac"
+            and  c1: "(tc,tc') \<in> step\<^sub>c ac"
+          have "sc' \<sim>\<^sub>c d \<sim>\<^sub>c tc'"
+          proof(cases "sim_a ac = None")
+            assume "sim_a ac = None"
+            then have " sc' \<sim> sa \<and> tc' \<sim> ta"
+              using b0 b1 b4 b5 c0 c1 none_refine by blast
+            with b2 show ?thesis
+              by (meson b4 b5 sim_ifs)
+          next
+            assume "\<not> sim_a ac = None"
+            then have "\<exists>aa. sim_a ac = Some aa" by auto
+            then obtain aa where d0: "sim_a ac = Some aa" by auto
+            from b2 b4 b5 have d1: "sa \<sim>\<^sub>a d \<sim>\<^sub>a ta"
+              using b4 b5 sim_ifs by blast
+          from d0 have d2 : "domain\<^sub>c ac = domain\<^sub>a aa"
+            using dom_refine by blast
+          then have d3: " domain\<^sub>c ac \<leadsto>\<^sub>c d =  domain\<^sub>a aa \<leadsto>\<^sub>c d"
+            by (simp add: intefere_same)
+          from b2 b4 b5 have d4 : "sc \<sim>\<^sub>c domain\<^sub>c ac \<sim>\<^sub>c tc = sa \<sim>\<^sub>a domain\<^sub>a aa \<sim>\<^sub>a ta"
+            using d2 sim_ifs by auto
+          from b3 have d5: " domain\<^sub>a aa \<leadsto>\<^sub>a d \<longrightarrow> sa \<sim>\<^sub>a domain\<^sub>a aa \<sim>\<^sub>a ta"
+            using d2 d4 intefere_same by fastforce
+          have "\<exists>sa' ta'. sc' \<sim> sa' \<and> tc' \<sim> ta' \<and> (sa, sa') \<in> step\<^sub>a aa \<and> (ta, ta') \<in> step\<^sub>a aa"
+            using action_refine b0 b1 b4 b5 c0 c1 d0 by blast
+          then obtain sa' ta' where d6: "sc' \<sim> sa' \<and> tc' \<sim> ta' \<and> (sa, sa') \<in> step\<^sub>a aa \<and> (ta, ta') \<in> step\<^sub>a aa"
+            by auto
+          with a1 d1 d2 d3 d5 b4 b5 have "sa' \<sim>\<^sub>a d \<sim>\<^sub>a ta'" by blast
+          then show ?thesis
+            using d6 sim_ifs by blast
+        qed
+        }
+        then show ?thesis by blast
+      qed
+    }
+    then show ?thesis by blast
+  qed
+  then show ?thesis
+    using SM_IFS\<^sub>c.weak_step_consistent_def by fastforce
+qed
+
+end
+*)
+(*
+locale SM_Refine = 
+  SM_IFS\<^sub>c: SM_IFS s0\<^sub>c step\<^sub>c domain\<^sub>c obs\<^sub>c vpeq\<^sub>c interference\<^sub>c +
+  SM_IFS\<^sub>a: SM_IFS s0\<^sub>a step\<^sub>a domain\<^sub>a obs\<^sub>a vpeq\<^sub>a interference\<^sub>a
+  for s0\<^sub>c :: "'s\<^sub>c"
+  and step\<^sub>c :: "'a\<^sub>c \<Rightarrow> ('s\<^sub>c \<times> 's\<^sub>c) set"
+  and domain\<^sub>c :: "'a\<^sub>c \<Rightarrow> 'd"
+  and obs\<^sub>c :: "'s\<^sub>c \<Rightarrow> 'd \<Rightarrow> 'o\<^sub>c" (infixl "\<guillemotright>\<^sub>c"  55)
+  and vpeq\<^sub>c :: "'s\<^sub>c \<Rightarrow> 'd \<Rightarrow> 's\<^sub>c \<Rightarrow> bool" ("(_ \<sim>\<^sub>c_\<sim>\<^sub>c _)" [70,69,70] 60)
+  and interference\<^sub>c :: "'d \<Rightarrow> 'd \<Rightarrow> bool" ("(_ \<leadsto>\<^sub>c _)" [70,71] 60)
+  and s0\<^sub>a :: "'s\<^sub>a"
+  and step\<^sub>a :: "'a\<^sub>a \<Rightarrow> ('s\<^sub>a \<times> 's\<^sub>a) set"
+  and domain\<^sub>a :: "'a\<^sub>a \<Rightarrow> 'd"
+  and obs\<^sub>a :: "'s\<^sub>a \<Rightarrow> 'd \<Rightarrow> 'o\<^sub>a" (infixl "\<guillemotright>\<^sub>a"  55)
+  and vpeq\<^sub>a :: "'s\<^sub>a \<Rightarrow> 'd \<Rightarrow> 's\<^sub>a \<Rightarrow> bool" ("(_ \<sim>\<^sub>a_\<sim>\<^sub>a _)" [70,69,70] 60)
+  and interference\<^sub>a :: "'d \<Rightarrow> 'd \<Rightarrow> bool" ("(_ \<leadsto>\<^sub>a _)" [70,71] 60) + 
+fixes sim_s :: "'s\<^sub>c \<Rightarrow> 's\<^sub>a"
+assumes
+  init_sim : "sim_s s0\<^sub>c = s0\<^sub>a" and
+  action_refine : "SM_IFS\<^sub>c.reachable0 s\<^sub>c  \<longrightarrow> (s\<^sub>c, t\<^sub>c) \<in> step\<^sub>c a\<^sub>c \<longrightarrow> 
+                  (\<forall>sc sc'. (sc, sc') \<in> step\<^sub>c a\<^sub>c \<longrightarrow> sim_s sc = sim_s sc') \<or> 
+                  (\<exists>a\<^sub>a. \<forall>sc sc'. ((sc, sc') \<in> step\<^sub>c a\<^sub>c \<longrightarrow> (sim_s sc, sim_s sc') \<in> step\<^sub>a a\<^sub>a) 
+                  \<and> domain\<^sub>c a\<^sub>c = domain\<^sub>a a\<^sub>a)" and
+  intefere_same : "interference\<^sub>c = interference\<^sub>a" and 
   sim_ifs : "  (sim_s s\<^sub>c) \<sim>\<^sub>a d \<sim>\<^sub>a (sim_s t\<^sub>c) = s\<^sub>c \<sim>\<^sub>c d \<sim>\<^sub>c t\<^sub>c" 
 begin 
+
 
 abbreviation reachable0\<^sub>c :: "'s\<^sub>c \<Rightarrow> bool"
   where "reachable0\<^sub>c \<equiv> SM_IFS\<^sub>c.reachable0"
@@ -58,7 +280,7 @@ proof -
           fix s s'
           assume b0: "reachable0\<^sub>a (sim_s s) \<and> reachable0\<^sub>c  s \<and> s' \<in> execute\<^sub>c (b # bs) s"
           have b1: "\<forall>s1. (s, s1) \<in> step\<^sub>c b \<longrightarrow> reachable0\<^sub>a (sim_s s1)"
-            by (metis SM_IFS\<^sub>a.reachableStep action_refine b0 none_refine option.exhaust)
+            by (metis SM_IFS\<^sub>a.reachableStep action_refine b0)
           from b0 have "\<exists>s1. (s,s1)\<in> step\<^sub>c b \<and>  (s1 , s') \<in> run\<^sub>c bs"   
             using SM_IFS\<^sub>c.execute_def by auto
           then obtain s1 where b2: "(s,s1)\<in> step\<^sub>c b \<and>  (s1 , s') \<in> run\<^sub>c bs" by auto
@@ -79,7 +301,6 @@ lemma reachR_reach: "reachable0\<^sub>c sc \<Longrightarrow> reachable0\<^sub>a 
   by (metis Image_singleton_iff SM_IFS.execute_def SM_IFS\<^sub>a.reachableC0 SM_IFS\<^sub>c.SM_IFS_axioms 
      SM_IFS\<^sub>c.reachable0_def SM_IFS\<^sub>c.reachableC0 SM_IFS\<^sub>c.reachable_def init_sim reachR_reach1)
 
-thm SM_IFS\<^sub>a.local_respect_def
 
 theorem abs_lr_imp : "SM_IFS\<^sub>a.local_respect \<Longrightarrow> SM_IFS\<^sub>c.local_respect"
 proof-
@@ -96,35 +317,26 @@ proof-
         and  b1: "\<not> domain\<^sub>c ac \<leadsto>\<^sub>a d"
         and  b2: "(sc, sc') \<in> step\<^sub>c ac "
       have "sc \<sim>\<^sub>c d \<sim>\<^sub>c sc'"
-      proof(cases "sim_a ac = None")
-        assume c0: "sim_a ac = None"
-        with b2 have "sim_s sc = sim_s sc'" by (meson none_refine)
+      proof(cases "\<forall>sc sc'. (sc, sc') \<in> step\<^sub>c ac \<longrightarrow> sim_s sc = sim_s sc'")
+        assume  "\<forall>sc sc'. (sc, sc') \<in> step\<^sub>c ac \<longrightarrow> sim_s sc = sim_s sc'"
         then show ?thesis
-          by (metis SM_IFS\<^sub>c.vpeq_reflexive sim_ifs)
+          by (metis SM_IFS\<^sub>c.vpeq_reflexive b2 sim_ifs)
       next
-        assume d0: "\<not> sim_a ac = None"
-        then have  "\<exists>aa. sim_a ac = Some aa" by auto
-        then obtain aa where d1: "sim_a ac = Some aa" by force
-        then have d01: "domain\<^sub>c ac = domain\<^sub>a aa"
-          by (simp add: dom_refine)
-        with b1 have d2 :"\<not> domain\<^sub>c ac \<leadsto>\<^sub>a d"
-          by (simp add: intefere_same)
-        from b0 have d3: "reachable0\<^sub>a (sim_s sc)" by (simp add: reachR_reach)
-        from b2 have d4: "(sim_s sc, sim_s sc') \<in> step\<^sub>a aa"
-          using action_refine d1 by blast
-        with a1 d2 d3 have "sim_s sc \<sim>\<^sub>a d \<sim>\<^sub>a sim_s sc'"
-          by (simp add: d01)
-        then show ?thesis 
-          using sim_ifs by blast
+        assume d0: "\<not> (\<forall>sc sc'. (sc, sc') \<in> step\<^sub>c ac \<longrightarrow> sim_s sc = sim_s sc')"
+        then have "\<exists>aa. (sim_s sc, sim_s sc') \<in> step\<^sub>a aa \<and> domain\<^sub>c ac = domain\<^sub>a aa"
+          using action_refine b0 b2 by blast
+        then obtain aa where d1: "(sim_s sc, sim_s sc') \<in> step\<^sub>a aa \<and> domain\<^sub>c ac = domain\<^sub>a aa" by auto
+        with b1 have d2: "\<not> domain\<^sub>a aa \<leadsto>\<^sub>a d" by simp
+        from b0 have d3: "reachable0\<^sub>a (sim_s sc)" using reachR_reach by auto
+        with a1 d1 d2 have "sim_s sc \<sim>\<^sub>a d \<sim>\<^sub>a sim_s sc'" by blast
+        then show ?thesis by (simp add: sim_ifs)
       qed
     }
     then show ?thesis by auto
   qed
   then show ?thesis 
-    using SM_IFS\<^sub>c.local_respect_def intefere_same by blast
+    using SM_IFS\<^sub>c.local_respect_def intefere_same by blast 
 qed
-
-thm SM_IFS\<^sub>a.weak_step_consistent_def
 
 theorem abs_wsc_imp : "SM_IFS\<^sub>a.weak_step_consistent \<Longrightarrow> SM_IFS\<^sub>c.weak_step_consistent"
 proof-
@@ -150,32 +362,31 @@ proof-
           assume c0: "(sc,sc') \<in> step\<^sub>c ac"
             and  c1: "(tc,tc') \<in> step\<^sub>c ac"
           have "sc' \<sim>\<^sub>c d \<sim>\<^sub>c tc'"
-          proof(cases "sim_a ac = None")
-            assume "sim_a ac = None"
+          proof(cases "\<forall>sc sc'. (sc, sc') \<in> step\<^sub>c ac \<longrightarrow> sim_s sc = sim_s sc'")
+            assume "\<forall>sc sc'. (sc, sc') \<in> step\<^sub>c ac \<longrightarrow> sim_s sc = sim_s sc'"
             then have "sim_s sc' = sim_s sc \<and> sim_s tc' = sim_s tc"
-              using c0 c1 none_refine by force
+              using c0 c1  by force
             with b2 show ?thesis by (metis b2 sim_ifs)
           next
-            assume "\<not> sim_a ac = None"
-            then have "\<exists>aa. sim_a ac = Some aa" by auto
-            then obtain aa where d0: "sim_a ac = Some aa" by auto
+            assume "\<not> (\<forall>sc sc'. (sc, sc') \<in> step\<^sub>c ac \<longrightarrow> sim_s sc = sim_s sc')"
+            then have "\<exists>aa. (sim_s sc, sim_s sc') \<in> step\<^sub>a aa \<and> (sim_s tc, sim_s tc') \<in> step\<^sub>a aa \<and> domain\<^sub>c ac = domain\<^sub>a aa" 
+              by (meson action_refine b1 c0 c1)
+            then obtain aa where d0: "(sim_s sc, sim_s sc') \<in> step\<^sub>a aa \<and> (sim_s tc, sim_s tc') \<in> step\<^sub>a aa \<and> domain\<^sub>c ac = domain\<^sub>a aa" by auto
             from b0 have d1: "reachable0\<^sub>a (sim_s sc)"
               by (simp add: reachR_reach)
             from b1 have d2: "reachable0\<^sub>a (sim_s tc)"
               by (simp add: reachR_reach)
             from b2 have d3: "sim_s sc \<sim>\<^sub>a d \<sim>\<^sub>a sim_s tc"
               using sim_ifs by blast
-          from d0 have d5 : "domain\<^sub>c ac = domain\<^sub>a aa"
-            using dom_refine by blast
-          then have d6: " domain\<^sub>c ac \<leadsto>\<^sub>c d =  domain\<^sub>a aa \<leadsto>\<^sub>c d"
+            from d0 have d5: " domain\<^sub>c ac \<leadsto>\<^sub>c d =  domain\<^sub>a aa \<leadsto>\<^sub>c d"
             by (simp add: intefere_same)
-          from d5 have d7 : "sc \<sim>\<^sub>c domain\<^sub>c ac \<sim>\<^sub>c tc = sim_s sc \<sim>\<^sub>a domain\<^sub>a aa \<sim>\<^sub>a sim_s tc"
+          from d0 have d6 : "sc \<sim>\<^sub>c domain\<^sub>c ac \<sim>\<^sub>c tc = sim_s sc \<sim>\<^sub>a domain\<^sub>a aa \<sim>\<^sub>a sim_s tc"
             using sim_ifs by auto
-          with b3 d6 have d8: " domain\<^sub>a aa \<leadsto>\<^sub>a d \<longrightarrow> sim_s sc \<sim>\<^sub>a domain\<^sub>a aa \<sim>\<^sub>a sim_s tc"
+          with b3 d5 have d7: " domain\<^sub>a aa \<leadsto>\<^sub>a d \<longrightarrow> sim_s sc \<sim>\<^sub>a domain\<^sub>a aa \<sim>\<^sub>a sim_s tc"
             using intefere_same by fastforce
           from c0 c1 have "(sim_s sc, sim_s sc') \<in> step\<^sub>a aa \<and> (sim_s tc, sim_s tc') \<in> step\<^sub>a aa"
             using action_refine d0 by blast
-          with a1 d1 d2 d3 d8 have "sim_s sc' \<sim>\<^sub>ad\<sim>\<^sub>a sim_s tc'"  by blast
+          with a1 d1 d2 d3 d7 have "sim_s sc' \<sim>\<^sub>ad\<sim>\<^sub>a sim_s tc'"  by blast
           then show ?thesis
             using sim_ifs by blast
         qed
@@ -188,11 +399,8 @@ proof-
   then show ?thesis
     using SM_IFS\<^sub>c.weak_step_consistent_def by fastforce
 qed
-
-
+*)
 end
 
-
-end
 
 
