PiCore_Refine.thy
@@ -2,8 +2,6 @@ theory PiCore_Refine
   imports PiCore_IFS Refinement
 begin
 
-print_locale InfoFlow
-
 locale PiCore_Refine =
   InfoFlow\<^sub>c: InfoFlow ptran\<^sub>c petran\<^sub>c fin_com\<^sub>c C0\<^sub>c step\<^sub>c interference\<^sub>c vpeq\<^sub>c obs\<^sub>c dome\<^sub>c +
   InfoFlow\<^sub>a: InfoFlow ptran\<^sub>a petran\<^sub>a fin_com\<^sub>a C0\<^sub>a step\<^sub>a interference\<^sub>a vpeq\<^sub>a obs\<^sub>a dome\<^sub>a
@@ -13,7 +11,7 @@ locale PiCore_Refine =
   and C0\<^sub>c  :: "('l\<^sub>c,'k\<^sub>c,'s\<^sub>c,'prog\<^sub>c) pesconf"
   and step\<^sub>c :: "('l\<^sub>c,'k\<^sub>c,'s\<^sub>c,'prog\<^sub>c, 'd) action \<Rightarrow> (('l\<^sub>c,'k\<^sub>c,'s\<^sub>c,'prog\<^sub>c) pesconf \<times> ('l\<^sub>c,'k\<^sub>c,'s\<^sub>c,'prog\<^sub>c) pesconf) set"
   and interference\<^sub>c :: "'d \<Rightarrow> 'd \<Rightarrow> bool" 
-  and vpeq\<^sub>c :: "'s\<^sub>c \<Rightarrow> 'd \<Rightarrow> 's\<^sub>c \<Rightarrow> bool" 
+  and vpeq\<^sub>c :: "'s\<^sub>c \<Rightarrow> 'd \<Rightarrow> 's\<^sub>c \<Rightarrow> bool" ("(_ \<sim>\<^sub>c_\<sim>\<^sub>c _)" [70,69,70] 60)
   and obs\<^sub>c :: "'s\<^sub>c \<Rightarrow> 'd \<Rightarrow> 'o\<^sub>c" 
   and dome\<^sub>c :: "'s\<^sub>c \<Rightarrow> ('l\<^sub>c, 'k\<^sub>c, 's\<^sub>c, 'prog\<^sub>c) event \<Rightarrow> 'd"
   and ptran\<^sub>a :: "'Env\<^sub>a \<Rightarrow> (('prog\<^sub>a \<times> 's\<^sub>a) \<times> 'prog\<^sub>a \<times> 's\<^sub>a) set"
@@ -22,21 +20,22 @@ locale PiCore_Refine =
   and C0\<^sub>a :: "('l\<^sub>a, 'k\<^sub>a, 's\<^sub>a, 'prog\<^sub>a) pesconf"
   and step\<^sub>a :: "('l\<^sub>a,'k\<^sub>a,'s\<^sub>a,'prog\<^sub>a, 'd) action \<Rightarrow> (('l\<^sub>a,'k\<^sub>a,'s\<^sub>a,'prog\<^sub>a) pesconf \<times> ('l\<^sub>a,'k\<^sub>a,'s\<^sub>a,'prog\<^sub>a) pesconf) set" 
   and interference\<^sub>a :: "'d \<Rightarrow> 'd \<Rightarrow> bool" 
-  and vpeq\<^sub>a ::  "'s\<^sub>a \<Rightarrow> 'd \<Rightarrow> 's\<^sub>a \<Rightarrow> bool"
+  and vpeq\<^sub>a ::  "'s\<^sub>a \<Rightarrow> 'd \<Rightarrow> 's\<^sub>a \<Rightarrow> bool" ("(_ \<sim>\<^sub>a_\<sim>\<^sub>a _)" [70,69,70] 60)
   and obs\<^sub>a :: "'s\<^sub>a \<Rightarrow> 'd \<Rightarrow> 'o\<^sub>a" 
   and dome\<^sub>a :: "'s\<^sub>a \<Rightarrow> ('l\<^sub>a, 'k\<^sub>a, 's\<^sub>a, 'prog\<^sub>a) event \<Rightarrow> 'd" +
-fixes sim_s ::  "('l\<^sub>c,'k\<^sub>c,'s\<^sub>c,'prog\<^sub>c) pesconf \<Rightarrow> ('l\<^sub>a, 'k\<^sub>a, 's\<^sub>a, 'prog\<^sub>a) pesconf"
+fixes sim_s ::  "('l\<^sub>c,'k\<^sub>c,'s\<^sub>c,'prog\<^sub>c) pesconf \<Rightarrow> ('l\<^sub>a, 'k\<^sub>a, 's\<^sub>a, 'prog\<^sub>a) pesconf \<Rightarrow> bool" ("(_ \<sim> _)" [70,70] 60)
   and sim_a :: "('l\<^sub>c, 'k\<^sub>c, 's\<^sub>c, 'prog\<^sub>c, 'd) action \<Rightarrow> ('l\<^sub>a, 'k\<^sub>a, 's\<^sub>a, 'prog\<^sub>a, 'd) action option"
 assumes
-  init_sim : "sim_s C0\<^sub>c = C0\<^sub>a" and
-  action_refine : "sim_a a\<^sub>c = Some a\<^sub>a \<longrightarrow> (C\<^sub>c, C'\<^sub>c) \<in> step\<^sub>c a\<^sub>c \<longrightarrow> (sim_s C\<^sub>c, sim_s C'\<^sub>c) \<in> step\<^sub>a a\<^sub>a" and
-  none_refine : "sim_a a\<^sub>c = None \<longrightarrow> (C\<^sub>c, C'\<^sub>c) \<in> step\<^sub>c a\<^sub>c \<longrightarrow> sim_s C\<^sub>c = sim_s C'\<^sub>c" and
+  init_sim : " C0\<^sub>c \<sim> C0\<^sub>a" and
+  action_refine : "\<lbrakk>sim_a a\<^sub>c = Some a\<^sub>a; InfoFlow\<^sub>c.reachablec0 C\<^sub>c; C\<^sub>c \<sim> C\<^sub>a; (C\<^sub>c, C\<^sub>c') \<in> step\<^sub>c a\<^sub>c\<rbrakk> \<Longrightarrow> 
+                   \<exists>C\<^sub>a'. C\<^sub>c' \<sim> C\<^sub>a' \<and> (C\<^sub>a, C\<^sub>a') \<in> step\<^sub>a a\<^sub>a" and
+  none_refine : "\<lbrakk>sim_a a\<^sub>c = None; InfoFlow\<^sub>c.reachablec0 C\<^sub>c; C\<^sub>c \<sim> C\<^sub>a; (C\<^sub>c, C\<^sub>c') \<in> step\<^sub>c a\<^sub>c\<rbrakk> \<Longrightarrow> C\<^sub>c' \<sim> C\<^sub>a" and
   intefere_same : "interference\<^sub>c  = interference\<^sub>a" and 
   dom_refine : "sim_a a\<^sub>c = Some a\<^sub>a \<longrightarrow> domain a\<^sub>c = domain a\<^sub>a" and 
-  sim_ifs : "vpeq\<^sub>a (gets (sim_s C\<^sub>c)) d (gets (sim_s C'\<^sub>c)) = vpeq\<^sub>c (gets C\<^sub>c) d (gets C'\<^sub>c)"   
-
+  sim_ifs : "\<lbrakk>C\<^sub>c \<sim> C\<^sub>a; T\<^sub>c \<sim> T\<^sub>a\<rbrakk> \<Longrightarrow>  (gets C\<^sub>a) \<sim>\<^sub>a d \<sim>\<^sub>a (gets T\<^sub>a) = (gets C\<^sub>c) \<sim>\<^sub>c d \<sim>\<^sub>c (gets T\<^sub>c)" 
 begin
 
+thm action_refine
 definition vpeqc :: "('l\<^sub>c,'k\<^sub>c,'s\<^sub>c,'prog\<^sub>c) pesconf \<Rightarrow> 'd \<Rightarrow> ('l\<^sub>c,'k\<^sub>c,'s\<^sub>c,'prog\<^sub>c) pesconf \<Rightarrow> bool" 
    where "vpeqc C1 u C2 \<equiv> vpeq\<^sub>c (gets C1) u (gets C2)"
 
@@ -65,16 +64,92 @@ proof
     using InfoFlow\<^sub>a.vpeqC_symmetric by force
   show "\<forall>a u. InfoFlow\<^sub>a.vpeqC a u a"
     using InfoFlow\<^sub>a.vpeqC_reflexive by blast
-  show "sim_s C0\<^sub>c = C0\<^sub>a"
+  show "C0\<^sub>c \<sim> C0\<^sub>a"
     by (simp add: init_sim)
-  show "\<And>a\<^sub>c a\<^sub>a s\<^sub>c t\<^sub>c. sim_a a\<^sub>c = Some a\<^sub>a \<longrightarrow> (s\<^sub>c, t\<^sub>c) \<in> step\<^sub>c a\<^sub>c \<longrightarrow> (sim_s s\<^sub>c, sim_s t\<^sub>c) \<in> step\<^sub>a a\<^sub>a"
-    by (simp add: action_refine)
-  show "\<And>a\<^sub>c s\<^sub>c t\<^sub>c. sim_a a\<^sub>c = None \<longrightarrow> (s\<^sub>c, t\<^sub>c) \<in> step\<^sub>c a\<^sub>c \<longrightarrow> sim_s s\<^sub>c = sim_s t\<^sub>c"
-    by (simp add: none_refine)
+  show " \<And>a\<^sub>c a\<^sub>a s\<^sub>c s\<^sub>a t\<^sub>c. sim_a a\<^sub>c = Some a\<^sub>a \<Longrightarrow> SM_IFS.reachable0 C0\<^sub>c step\<^sub>c s\<^sub>c \<Longrightarrow> s\<^sub>c \<sim> s\<^sub>a \<Longrightarrow> 
+        (s\<^sub>c, t\<^sub>c) \<in> step\<^sub>c a\<^sub>c \<Longrightarrow> \<exists>t\<^sub>a. t\<^sub>c \<sim> t\<^sub>a \<and> (s\<^sub>a, t\<^sub>a) \<in> step\<^sub>a a\<^sub>a"
+    using InfoFlow\<^sub>c.reachable0_equiv action_refine by blast
+  show "\<And>a\<^sub>c s\<^sub>c s\<^sub>a t\<^sub>c. sim_a a\<^sub>c = None \<Longrightarrow> SM_IFS.reachable0 C0\<^sub>c step\<^sub>c s\<^sub>c \<Longrightarrow> s\<^sub>c \<sim> s\<^sub>a \<Longrightarrow> (s\<^sub>c, t\<^sub>c) \<in> step\<^sub>c a\<^sub>c \<Longrightarrow> t\<^sub>c \<sim> s\<^sub>a"
+    using InfoFlow\<^sub>c.reachable0_equiv none_refine by blast
   show "interference\<^sub>c = interference\<^sub>a"
     using  intefere_same by force
   show "\<And>a\<^sub>c a\<^sub>a. sim_a a\<^sub>c = Some a\<^sub>a \<longrightarrow> domain a\<^sub>c = domain a\<^sub>a"
     by (simp add:  dom_refine)
+  show " \<And>s\<^sub>c s\<^sub>a t\<^sub>c t\<^sub>a d. s\<^sub>c \<sim> s\<^sub>a \<Longrightarrow> t\<^sub>c \<sim> t\<^sub>a \<Longrightarrow> InfoFlow\<^sub>a.vpeqC s\<^sub>a d t\<^sub>a = InfoFlow\<^sub>c.vpeqC s\<^sub>c d t\<^sub>c"
+    by (simp add: InfoFlow\<^sub>a.vpeqC_def InfoFlow\<^sub>c.vpeqC_def sim_ifs)
+qed
+
+theorem PiCore_abs_lr_imp: "InfoFlow\<^sub>a.local_respectC \<Longrightarrow> InfoFlow\<^sub>c.local_respectC"
+  using InfoFlow\<^sub>a.local_respectC_equiv InfoFlow\<^sub>c.local_respectC_equiv abs_lr_imp by blast
+
+theorem PiCore_abs_wsc_imp: "InfoFlow\<^sub>a.weak_step_consistentC \<Longrightarrow> InfoFlow\<^sub>c.weak_step_consistentC"
+  using InfoFlow\<^sub>a.weak_step_consistentC_equiv InfoFlow\<^sub>c.weak_step_consistentC_equiv abs_wsc_imp by fastforce
+
+end
+
+(*
+locale PiCore_Refine =
+  InfoFlow\<^sub>c: InfoFlow ptran\<^sub>c petran\<^sub>c fin_com\<^sub>c C0\<^sub>c step\<^sub>c interference\<^sub>c vpeq\<^sub>c obs\<^sub>c dome\<^sub>c +
+  InfoFlow\<^sub>a: InfoFlow ptran\<^sub>a petran\<^sub>a fin_com\<^sub>a C0\<^sub>a step\<^sub>a interference\<^sub>a vpeq\<^sub>a obs\<^sub>a dome\<^sub>a
+  for ptran\<^sub>c :: "'Env\<^sub>c \<Rightarrow> (('prog\<^sub>c \<times> 's\<^sub>c) \<times> 'prog\<^sub>c \<times> 's\<^sub>c) set" 
+  and petran\<^sub>c :: "'Env\<^sub>c \<Rightarrow> 'prog\<^sub>c \<times> 's\<^sub>c \<Rightarrow> 'prog\<^sub>c \<times> 's\<^sub>c \<Rightarrow> bool" 
+  and fin_com\<^sub>c :: "'prog\<^sub>c"
+  and C0\<^sub>c  :: "('l\<^sub>c,'k\<^sub>c,'s\<^sub>c,'prog\<^sub>c) pesconf"
+  and step\<^sub>c :: "('l\<^sub>c,'k\<^sub>c,'s\<^sub>c,'prog\<^sub>c, 'd) action \<Rightarrow> (('l\<^sub>c,'k\<^sub>c,'s\<^sub>c,'prog\<^sub>c) pesconf \<times> ('l\<^sub>c,'k\<^sub>c,'s\<^sub>c,'prog\<^sub>c) pesconf) set"
+  and interference\<^sub>c :: "'d \<Rightarrow> 'd \<Rightarrow> bool" 
+  and vpeq\<^sub>c :: "'s\<^sub>c \<Rightarrow> 'd \<Rightarrow> 's\<^sub>c \<Rightarrow> bool" ("(_ \<sim>\<^sub>c_\<sim>\<^sub>c _)" [70,69,70] 60)
+  and obs\<^sub>c :: "'s\<^sub>c \<Rightarrow> 'd \<Rightarrow> 'o\<^sub>c" 
+  and dome\<^sub>c :: "'s\<^sub>c \<Rightarrow> ('l\<^sub>c, 'k\<^sub>c, 's\<^sub>c, 'prog\<^sub>c) event \<Rightarrow> 'd"
+  and ptran\<^sub>a :: "'Env\<^sub>a \<Rightarrow> (('prog\<^sub>a \<times> 's\<^sub>a) \<times> 'prog\<^sub>a \<times> 's\<^sub>a) set"
+  and petran\<^sub>a :: "'Env\<^sub>a \<Rightarrow> 'prog\<^sub>a \<times> 's\<^sub>a \<Rightarrow> 'prog\<^sub>a \<times> 's\<^sub>a \<Rightarrow> bool" 
+  and fin_com\<^sub>a :: "'prog\<^sub>a"
+  and C0\<^sub>a :: "('l\<^sub>a, 'k\<^sub>a, 's\<^sub>a, 'prog\<^sub>a) pesconf"
+  and step\<^sub>a :: "('l\<^sub>a,'k\<^sub>a,'s\<^sub>a,'prog\<^sub>a, 'd) action \<Rightarrow> (('l\<^sub>a,'k\<^sub>a,'s\<^sub>a,'prog\<^sub>a) pesconf \<times> ('l\<^sub>a,'k\<^sub>a,'s\<^sub>a,'prog\<^sub>a) pesconf) set" 
+  and interference\<^sub>a :: "'d \<Rightarrow> 'd \<Rightarrow> bool" 
+  and vpeq\<^sub>a ::  "'s\<^sub>a \<Rightarrow> 'd \<Rightarrow> 's\<^sub>a \<Rightarrow> bool" ("(_ \<sim>\<^sub>a_\<sim>\<^sub>a _)" [70,69,70] 60)
+  and obs\<^sub>a :: "'s\<^sub>a \<Rightarrow> 'd \<Rightarrow> 'o\<^sub>a" 
+  and dome\<^sub>a :: "'s\<^sub>a \<Rightarrow> ('l\<^sub>a, 'k\<^sub>a, 's\<^sub>a, 'prog\<^sub>a) event \<Rightarrow> 'd" +
+fixes sim_s ::  "('l\<^sub>c,'k\<^sub>c,'s\<^sub>c,'prog\<^sub>c) pesconf \<Rightarrow> ('l\<^sub>a, 'k\<^sub>a, 's\<^sub>a, 'prog\<^sub>a) pesconf"
+  and sim_a :: "('l\<^sub>c, 'k\<^sub>c, 's\<^sub>c, 'prog\<^sub>c, 'd) action \<Rightarrow> ('l\<^sub>a, 'k\<^sub>a, 's\<^sub>a, 'prog\<^sub>a, 'd) action option"
+assumes
+  init_sim : "sim_s C0\<^sub>c = C0\<^sub>a" and
+  action_refine : "InfoFlow\<^sub>c.reachablec0 C\<^sub>c \<longrightarrow> (C\<^sub>c, C\<^sub>c') \<in> step\<^sub>c a\<^sub>c \<longrightarrow>
+                  (\<forall>Cc Cc'. (Cc, Cc') \<in> step\<^sub>c a\<^sub>c \<longrightarrow> sim_s Cc = sim_s Cc') \<or>
+                  (\<exists>a\<^sub>a. \<forall>Cc Cc'. (Cc, Cc') \<in> step\<^sub>c a\<^sub>c \<longrightarrow> ((sim_s Cc, sim_s Cc') \<in> step\<^sub>a a\<^sub>a)
+                  \<and> domain a\<^sub>c = domain a\<^sub>a)" and
+  intefere_same : "interference\<^sub>c  = interference\<^sub>a" and 
+  sim_ifs : "gets (sim_s C\<^sub>c) \<sim>\<^sub>a d \<sim>\<^sub>a gets (sim_s C'\<^sub>c) = gets C\<^sub>c \<sim>\<^sub>c d \<sim>\<^sub>c gets C'\<^sub>c"   
+begin
+
+lemma "InfoFlow\<^sub>c.reachablec0 s\<^sub>c \<longrightarrow> (s\<^sub>c, t\<^sub>c) \<in> step\<^sub>c a\<^sub>c \<longrightarrow>
+                  (\<forall>sc sc'. (sc, sc') \<in> step\<^sub>c a\<^sub>c \<longrightarrow> sim_s sc = sim_s sc') \<or>
+                  (\<exists>a\<^sub>a. \<forall>sc sc'. (sc, sc') \<in> step\<^sub>c a\<^sub>c \<longrightarrow> ((sim_s sc, sim_s sc') \<in> step\<^sub>a a\<^sub>a)
+                  \<and> domain a\<^sub>c = domain a\<^sub>a)"
+  using action_refine by blast
+interpretation SM_Refine C0\<^sub>c step\<^sub>c domain InfoFlow\<^sub>c.obsC InfoFlow\<^sub>c.vpeqC interference\<^sub>c
+                         C0\<^sub>a step\<^sub>a domain InfoFlow\<^sub>a.obsC InfoFlow\<^sub>a.vpeqC interference\<^sub>a
+                         sim_s
+proof
+  show " \<forall>a b c u. InfoFlow\<^sub>c.vpeqC a u b \<and> InfoFlow\<^sub>c.vpeqC b u c \<longrightarrow> InfoFlow\<^sub>c.vpeqC a u c"
+    using InfoFlow\<^sub>c.vpeqC_transitive by force
+  show "\<forall>a b u. InfoFlow\<^sub>c.vpeqC a u b \<longrightarrow> InfoFlow\<^sub>c.vpeqC b u a"
+    using InfoFlow\<^sub>c.vpeqC_symmetric by blast
+  show " \<forall>a u. InfoFlow\<^sub>c.vpeqC a u a"
+    using InfoFlow\<^sub>c.vpeqC_reflexive by blast
+  show " \<forall>a b c u. InfoFlow\<^sub>a.vpeqC a u b \<and> InfoFlow\<^sub>a.vpeqC b u c \<longrightarrow> InfoFlow\<^sub>a.vpeqC a u c"
+    using InfoFlow\<^sub>a.vpeqC_transitive by fastforce
+  show "\<forall>a b u. InfoFlow\<^sub>a.vpeqC a u b \<longrightarrow> InfoFlow\<^sub>a.vpeqC b u a"
+    using InfoFlow\<^sub>a.vpeqC_symmetric by force
+  show "\<forall>a u. InfoFlow\<^sub>a.vpeqC a u a"
+    using InfoFlow\<^sub>a.vpeqC_reflexive by blast
+  show "sim_s C0\<^sub>c = C0\<^sub>a"
+    by (simp add: init_sim)
+  show "\<And>s\<^sub>c t\<^sub>c a\<^sub>c. SM_IFS.reachable0 C0\<^sub>c step\<^sub>c s\<^sub>c \<longrightarrow> (s\<^sub>c, t\<^sub>c) \<in> step\<^sub>c a\<^sub>c \<longrightarrow> 
+       (\<forall>sc sc'. (sc, sc') \<in> step\<^sub>c a\<^sub>c \<longrightarrow> sim_s sc = sim_s sc') \<or> (\<exists>a\<^sub>a. \<forall>sc sc'. ((sc, sc') \<in> step\<^sub>c a\<^sub>c 
+       \<longrightarrow> (sim_s sc, sim_s sc') \<in> step\<^sub>a a\<^sub>a) \<and> domain a\<^sub>c = domain a\<^sub>a)"
+    by (meson InfoFlow\<^sub>c.reachable0_equiv action_refine)
+  show "interference\<^sub>c = interference\<^sub>a"
+    using  intefere_same by force
   show "\<And>s\<^sub>c d t\<^sub>c. InfoFlow\<^sub>a.vpeqC (sim_s s\<^sub>c) d (sim_s t\<^sub>c) = InfoFlow\<^sub>c.vpeqC s\<^sub>c d t\<^sub>c"
     by (simp add: InfoFlow\<^sub>a.vpeqC_def InfoFlow\<^sub>c.vpeqC_def sim_ifs)
 qed
@@ -86,5 +161,6 @@ theorem PiCore_abs_wsc_imp: "InfoFlow\<^sub>a.weak_step_consistentC \<Longrighta
   using InfoFlow\<^sub>a.weak_step_consistentC_equiv InfoFlow\<^sub>c.weak_step_consistentC_equiv abs_wsc_imp by fastforce
 
 end
+*)
 
 end
