PiCore_Sim.thy
@@ -2,6 +2,13 @@ theory PiCore_Sim
   imports PiCore_Refine
 begin
 
+
+definition related_transitions:: "('s\<^sub>c \<times> 's\<^sub>c) set \<Rightarrow> ('s\<^sub>a \<times> 's\<^sub>a) set \<Rightarrow> ('s\<^sub>c \<times> 's\<^sub>a) set \<Rightarrow> 
+                                  (('s\<^sub>c \<times> 's\<^sub>c) \<times> ('s\<^sub>a \<times> 's\<^sub>a)) set" ("'(_, _')\<^sub>_")
+  where "related_transitions R R' \<alpha> = {((\<sigma>,\<sigma>'),(\<Sigma>,\<Sigma>')). (\<sigma>,\<sigma>')\<in> R \<and> (\<Sigma>,\<Sigma>')\<in>R' 
+                                      \<and>(\<sigma>, \<Sigma>) \<in> \<alpha> \<and> (\<sigma>', \<Sigma>') \<in> \<alpha>}"
+
+thm related_transitions_def
 locale event_sim_validity = 
    event\<^sub>c: event ptran\<^sub>c petran\<^sub>c fin_com\<^sub>c + 
    event\<^sub>a: event ptran\<^sub>a petran\<^sub>a fin_com\<^sub>a
@@ -10,18 +17,27 @@ and petran\<^sub>c :: "'Env\<^sub>c \<Rightarrow> ('s\<^sub>c,'prog\<^sub>c) pco
 and fin_com\<^sub>c :: "'prog\<^sub>c"
 and ptran\<^sub>a :: "'Env\<^sub>a \<Rightarrow> (('s\<^sub>a,'prog\<^sub>a) pconf \<times> ('s\<^sub>a,'prog\<^sub>a) pconf) set" 
 and petran\<^sub>a :: "'Env\<^sub>a \<Rightarrow> ('s\<^sub>a,'prog\<^sub>a) pconf \<Rightarrow> ('s\<^sub>a,'prog\<^sub>a) pconf \<Rightarrow> bool"
-and fin_com\<^sub>a :: "'prog\<^sub>a"
-+ fixes sim_s :: "'s\<^sub>c \<Rightarrow> 's\<^sub>a"
-  and   prog_sim :: "['Env\<^sub>c, ('s\<^sub>c,'prog\<^sub>c) pconf, ('s\<^sub>c \<times> 's\<^sub>c) set, ('s\<^sub>c \<times> 's\<^sub>c) set, 
-                      'Env\<^sub>a, ('s\<^sub>a,'prog\<^sub>a) pconf, ('s\<^sub>a \<times> 's\<^sub>a) set, ('s\<^sub>a \<times> 's\<^sub>a) set] \<Rightarrow> bool" 
-  ("'(_,_,_,_')/ \<preceq>\<^sub>p /'(_,_,_,_')" [81,81,81,81,81,81,81,81] 100)
-assumes prog_sim_validity: "(\<Gamma>\<^sub>c, (P\<^sub>c, s\<^sub>c), R\<^sub>c, G\<^sub>c) \<preceq>\<^sub>p (\<Gamma>\<^sub>a, (P\<^sub>a, s\<^sub>a), R\<^sub>a, G\<^sub>a) \<Longrightarrow> 
-        sim_s s\<^sub>c = s\<^sub>a \<and> 
-        (((P\<^sub>c, s\<^sub>c), (P'\<^sub>c, s'\<^sub>c)) \<in> ptran\<^sub>c \<Gamma>\<^sub>c  \<longrightarrow> (s\<^sub>c, s'\<^sub>c) \<in> G\<^sub>c \<longrightarrow>
-        ((\<Gamma>\<^sub>c, (P'\<^sub>c, s'\<^sub>c), R\<^sub>c, G\<^sub>c) \<preceq>\<^sub>p (\<Gamma>\<^sub>a, (P\<^sub>a, s\<^sub>a), R\<^sub>a, G\<^sub>a) \<or> 
-        ((P\<^sub>a, s\<^sub>a), (P'\<^sub>a, sim_s s'\<^sub>c)) \<in> ptran\<^sub>a \<Gamma>\<^sub>a \<and> (s\<^sub>a, sim_s s'\<^sub>c) \<in> G\<^sub>a \<and> 
-        (\<Gamma>\<^sub>c, (P'\<^sub>c, s'\<^sub>c), R\<^sub>c, G\<^sub>c) \<preceq>\<^sub>p (\<Gamma>\<^sub>a, (P'\<^sub>a, sim_s s'\<^sub>c), R\<^sub>a, G\<^sub>a)))"
+and fin_com\<^sub>a :: "'prog\<^sub>a" +
+fixes prog_sim :: "['Env\<^sub>c, ('s\<^sub>c,'prog\<^sub>c) pconf, ('s\<^sub>c \<times> 's\<^sub>c) set, ('s\<^sub>c \<times> 's\<^sub>c) set, 
+                  ('s\<^sub>c \<times> 's\<^sub>a) set, 'prog\<^sub>c \<Rightarrow> 'prog\<^sub>a option, ('s\<^sub>c \<times> 's\<^sub>a) set,
+                  'Env\<^sub>a, ('s\<^sub>a,'prog\<^sub>a) pconf, ('s\<^sub>a \<times> 's\<^sub>a) set, ('s\<^sub>a \<times> 's\<^sub>a) set] \<Rightarrow> bool" 
+  ("'(_,_,_,_')/ \<preceq>\<^sub>p \<^sub>'(\<^sub>_\<^sub>;\<^sub>_\<^sub>;\<^sub>_\<^sub>') /'(_,_,_,_')" [81,81,81,81,81,81,81,81,81,81,81] 100)
+assumes prog_sim_validity: "(\<Gamma>\<^sub>c, (P\<^sub>c, s\<^sub>c), R\<^sub>c, G\<^sub>c) \<preceq>\<^sub>p \<^sub>(\<^sub>\<alpha>\<^sub>;\<^sub>\<zeta>\<^sub>;\<^sub>\<gamma>\<^sub>) (\<Gamma>\<^sub>a, (P\<^sub>a, s\<^sub>a), R\<^sub>a, G\<^sub>a) \<Longrightarrow>
+                            (s\<^sub>c, s\<^sub>a) \<in> \<alpha> \<and>
+
+                            (((P\<^sub>c, s\<^sub>c), (P\<^sub>c', s\<^sub>c')) \<in> ptran\<^sub>c \<Gamma>\<^sub>c \<and> \<zeta> P\<^sub>c = None \<longrightarrow> (s\<^sub>c, s\<^sub>c') \<in> G\<^sub>c \<and> 
+                            (\<Gamma>\<^sub>c, (P\<^sub>c', s\<^sub>c'), R\<^sub>c, G\<^sub>c) \<preceq>\<^sub>p \<^sub>(\<^sub>\<alpha>\<^sub>;\<^sub>\<zeta>\<^sub>;\<^sub>\<gamma>\<^sub>) (\<Gamma>\<^sub>a, (P\<^sub>a, s\<^sub>a), R\<^sub>a, G\<^sub>a)) \<and>
+
+                            (((P\<^sub>c, s\<^sub>c), (P\<^sub>c', s\<^sub>c')) \<in> ptran\<^sub>c \<Gamma>\<^sub>c \<and> \<zeta> P\<^sub>c = Some P\<^sub>a \<longrightarrow> (\<exists>P\<^sub>a' s\<^sub>a'. 
+                            ((P\<^sub>a, s\<^sub>a), (P\<^sub>a', s\<^sub>a')) \<in> ptran\<^sub>a \<Gamma>\<^sub>a \<and> (s\<^sub>c, s\<^sub>c') \<in> G\<^sub>c \<and> (s\<^sub>a, s\<^sub>a') \<in> G\<^sub>a \<and>
+                            (\<Gamma>\<^sub>c, (P\<^sub>c', s\<^sub>c'), R\<^sub>c, G\<^sub>c) \<preceq>\<^sub>p \<^sub>(\<^sub>\<alpha>\<^sub>;\<^sub>\<zeta>\<^sub>;\<^sub>\<gamma>\<^sub>) (\<Gamma>\<^sub>a, (P\<^sub>a', s\<^sub>a'), R\<^sub>a, G\<^sub>a))) \<and>
+                      
+                            (P\<^sub>c = fin_com\<^sub>c \<longrightarrow> P\<^sub>a = fin_com\<^sub>a \<and> (s\<^sub>c, s\<^sub>a) \<in> \<gamma>) \<and> 
+
+                            (((s\<^sub>c, s\<^sub>c'), (s\<^sub>a, s\<^sub>a')) \<in> (R\<^sub>c, R\<^sub>a \<union> Id)\<^sub>\<alpha> \<longrightarrow> 
+                            (\<Gamma>\<^sub>c, (P\<^sub>c, s\<^sub>c'), R\<^sub>c, G\<^sub>c) \<preceq>\<^sub>p \<^sub>(\<^sub>\<alpha>\<^sub>;\<^sub>\<zeta>\<^sub>;\<^sub>\<gamma>\<^sub>) (\<Gamma>\<^sub>a, (P\<^sub>a, s\<^sub>a'), R\<^sub>a, G\<^sub>a))"
 begin
+
 
 abbreviation ptran\<^sub>c' :: "'Env\<^sub>c \<Rightarrow> ('s\<^sub>c,'prog\<^sub>c) pconf \<Rightarrow> ('s\<^sub>c,'prog\<^sub>c) pconf \<Rightarrow> bool" ("_ \<turnstile>\<^sub>c _ -c\<rightarrow> _" [81,81] 80)
   where "ptran\<^sub>c' \<equiv> event\<^sub>c.ptran'"
@@ -29,19 +45,19 @@ abbreviation ptran\<^sub>c' :: "'Env\<^sub>c \<Rightarrow> ('s\<^sub>c,'prog\<^s
 abbreviation ptrans\<^sub>c :: "'Env\<^sub>c \<Rightarrow> ('s\<^sub>c,'prog\<^sub>c) pconf \<Rightarrow> ('s\<^sub>c,'prog\<^sub>c) pconf \<Rightarrow> bool" ("_ \<turnstile>\<^sub>c _ c*\<rightarrow> _" [81,81] 80)
   where "ptrans\<^sub>c \<equiv> event\<^sub>c.ptrans"
 
-abbreviation etran\<^sub>c ::  "'Env\<^sub>c \<Rightarrow> ('l\<^sub>c,'k\<^sub>c,'s\<^sub>c,'prog\<^sub>c) econf \<Rightarrow> ('l\<^sub>c,'k\<^sub>c,'s\<^sub>c,'prog\<^sub>c) actk \<Rightarrow> 
-                        ('l\<^sub>c,'k\<^sub>c,'s\<^sub>c,'prog\<^sub>c) econf \<Rightarrow> bool" ("_ \<turnstile>\<^sub>c _ -et-_\<rightarrow> _" [81,81,81] 80)
+abbreviation etran\<^sub>c ::  "'Env\<^sub>c \<Rightarrow> ('l\<^sub>c,'k,'s\<^sub>c,'prog\<^sub>c) econf \<Rightarrow> ('l\<^sub>c,'k,'s\<^sub>c,'prog\<^sub>c) actk \<Rightarrow> 
+                        ('l\<^sub>c,'k,'s\<^sub>c,'prog\<^sub>c) econf \<Rightarrow> bool" ("_ \<turnstile>\<^sub>c _ -et-_\<rightarrow> _" [81,81,81] 80)
   where "etran\<^sub>c \<equiv> event\<^sub>c.etran"
 
-(*
-abbreviation estran\<^sub>c :: "'Env\<^sub>c \<Rightarrow> ('l\<^sub>c,'k\<^sub>c,'s\<^sub>c,'prog\<^sub>c) esconf \<Rightarrow> ('l\<^sub>c,'k\<^sub>c,'s\<^sub>c,'prog\<^sub>c) actk \<Rightarrow> 
-                        ('l\<^sub>c,'k\<^sub>c,'s\<^sub>c,'prog\<^sub>c) esconf \<Rightarrow> bool" ("_ \<turnstile>\<^sub>c _ -es-_\<rightarrow> _" [81,81] 80)
+
+abbreviation estran\<^sub>c :: "'Env\<^sub>c \<Rightarrow> ('l\<^sub>c,'k,'s\<^sub>c,'prog\<^sub>c) esconf \<Rightarrow> ('l\<^sub>c,'k,'s\<^sub>c,'prog\<^sub>c) actk \<Rightarrow> 
+                        ('l\<^sub>c,'k,'s\<^sub>c,'prog\<^sub>c) esconf \<Rightarrow> bool" ("_ \<turnstile>\<^sub>c _ -es-_\<rightarrow> _" [81,81] 80)
   where "estran\<^sub>c \<equiv> event\<^sub>c.estran"
 
-abbreviation pestran\<^sub>c :: "'Env\<^sub>c \<Rightarrow> ('l\<^sub>c,'k\<^sub>c,'s\<^sub>c,'prog\<^sub>c) pesconf \<Rightarrow> ('l\<^sub>c,'k\<^sub>c,'s\<^sub>c,'prog\<^sub>c) actk \<Rightarrow> 
-                        ('l\<^sub>c,'k\<^sub>c,'s\<^sub>c,'prog\<^sub>c) pesconf \<Rightarrow> bool" ("_ \<turnstile>\<^sub>c _ -pes-_\<rightarrow> _" [70,70] 60)
+abbreviation pestran\<^sub>c :: "'Env\<^sub>c \<Rightarrow> ('l\<^sub>c,'k,'s\<^sub>c,'prog\<^sub>c) pesconf \<Rightarrow> ('l\<^sub>c,'k,'s\<^sub>c,'prog\<^sub>c) actk \<Rightarrow> 
+                        ('l\<^sub>c,'k,'s\<^sub>c,'prog\<^sub>c) pesconf \<Rightarrow> bool" ("_ \<turnstile>\<^sub>c _ -pes-_\<rightarrow> _" [70,70] 60)
   where "pestran\<^sub>c \<equiv> event\<^sub>c.pestran"
-*)
+
 
 abbreviation ptran\<^sub>a' :: "'Env\<^sub>a \<Rightarrow> ('s\<^sub>a,'prog\<^sub>a) pconf \<Rightarrow> ('s\<^sub>a,'prog\<^sub>a) pconf \<Rightarrow> bool" ("_ \<turnstile>\<^sub>a _ -c\<rightarrow> _" [81,81] 80)
   where "ptran\<^sub>a' \<equiv> event\<^sub>a.ptran'"
@@ -49,64 +65,39 @@ abbreviation ptran\<^sub>a' :: "'Env\<^sub>a \<Rightarrow> ('s\<^sub>a,'prog\<^s
 abbreviation ptrans\<^sub>a :: "'Env\<^sub>a \<Rightarrow> ('s\<^sub>a,'prog\<^sub>a) pconf \<Rightarrow> ('s\<^sub>a,'prog\<^sub>a) pconf \<Rightarrow> bool" ("_ \<turnstile>\<^sub>a _ c*\<rightarrow> _" [81,81] 80)
   where "ptrans\<^sub>a \<equiv> event\<^sub>a.ptrans"
 
-abbreviation etran\<^sub>a ::  "'Env\<^sub>a \<Rightarrow> ('l\<^sub>a,'k\<^sub>a,'s\<^sub>a,'prog\<^sub>a) econf \<Rightarrow> ('l\<^sub>a,'k\<^sub>a,'s\<^sub>a,'prog\<^sub>a) actk \<Rightarrow> 
-                        ('l\<^sub>a,'k\<^sub>a,'s\<^sub>a,'prog\<^sub>a) econf \<Rightarrow> bool" ("_ \<turnstile>\<^sub>a _ -et-_\<rightarrow> _" [81,81,81] 80)
+abbreviation etran\<^sub>a ::  "'Env\<^sub>a \<Rightarrow> ('l\<^sub>a,'k,'s\<^sub>a,'prog\<^sub>a) econf \<Rightarrow> ('l\<^sub>a,'k,'s\<^sub>a,'prog\<^sub>a) actk \<Rightarrow> 
+                        ('l\<^sub>a,'k,'s\<^sub>a,'prog\<^sub>a) econf \<Rightarrow> bool" ("_ \<turnstile>\<^sub>a _ -et-_\<rightarrow> _" [81,81,81] 80)
   where "etran\<^sub>a \<equiv> event\<^sub>a.etran"
 
-(*
-abbreviation estran\<^sub>a :: "'Env\<^sub>a \<Rightarrow> ('l\<^sub>a,'k\<^sub>a,'s\<^sub>a,'prog\<^sub>a) esconf \<Rightarrow> ('l\<^sub>a,'k\<^sub>a,'s\<^sub>a,'prog\<^sub>a) actk \<Rightarrow> 
-                        ('l\<^sub>a,'k\<^sub>a,'s\<^sub>a,'prog\<^sub>a) esconf \<Rightarrow> bool" ("_ \<turnstile>\<^sub>a _ -es-_\<rightarrow> _" [81,81] 80)
+
+abbreviation estran\<^sub>a :: "'Env\<^sub>a \<Rightarrow> ('l\<^sub>a,'k,'s\<^sub>a,'prog\<^sub>a) esconf \<Rightarrow> ('l\<^sub>a,'k,'s\<^sub>a,'prog\<^sub>a) actk \<Rightarrow> 
+                        ('l\<^sub>a,'k,'s\<^sub>a,'prog\<^sub>a) esconf \<Rightarrow> bool" ("_ \<turnstile>\<^sub>a _ -es-_\<rightarrow> _" [81,81] 80)
   where "estran\<^sub>a \<equiv> event\<^sub>a.estran"
 
-abbreviation pestran\<^sub>a :: "'Env\<^sub>a \<Rightarrow> ('l\<^sub>a,'k\<^sub>a,'s\<^sub>a,'prog\<^sub>a) pesconf \<Rightarrow> ('l\<^sub>a,'k\<^sub>a,'s\<^sub>a,'prog\<^sub>a) actk \<Rightarrow> 
-                        ('l\<^sub>a,'k\<^sub>a,'s\<^sub>a,'prog\<^sub>a) pesconf \<Rightarrow> bool" ("_ \<turnstile>\<^sub>a _ -pes-_\<rightarrow> _" [70,70] 60)
+abbreviation pestran\<^sub>a :: "'Env\<^sub>a \<Rightarrow> ('l\<^sub>a,'k,'s\<^sub>a,'prog\<^sub>a) pesconf \<Rightarrow> ('l\<^sub>a,'k,'s\<^sub>a,'prog\<^sub>a) actk \<Rightarrow> 
+                        ('l\<^sub>a,'k,'s\<^sub>a,'prog\<^sub>a) pesconf \<Rightarrow> bool" ("_ \<turnstile>\<^sub>a _ -pes-_\<rightarrow> _" [70,70] 60)
   where "pestran\<^sub>a \<equiv> event\<^sub>a.pestran"
-*)
 
-inductive e_sim_validity :: "'Env\<^sub>c \<Rightarrow> ('l\<^sub>c,'k\<^sub>c,'s\<^sub>c,'prog\<^sub>c) econf \<Rightarrow> ('s\<^sub>c \<times> 's\<^sub>c) set \<Rightarrow> ('s\<^sub>c \<times> 's\<^sub>c) set
-    \<Rightarrow> 'Env\<^sub>a \<Rightarrow> ('l\<^sub>a,'k\<^sub>a,'s\<^sub>a,'prog\<^sub>a) econf \<Rightarrow> ('s\<^sub>a \<times> 's\<^sub>a) set \<Rightarrow> ('s\<^sub>a \<times> 's\<^sub>a) set \<Rightarrow> bool" 
-    ("'(_,_,_,_')/ \<preceq>\<^sub>e /'(_,_,_,_')" [81,81,81,81,81,81,81,81] 100)
-    where rgsim : "\<lbrakk>sim_s (gets_e econf\<^sub>c) = gets_e econf\<^sub>a ;
-                   \<forall>econf\<^sub>c' \<delta>\<^sub>c. (\<Gamma>\<^sub>c \<turnstile>\<^sub>c econf\<^sub>c -et-\<delta>\<^sub>c\<rightarrow>econf\<^sub>c') \<longrightarrow> 
-                   ((\<Gamma>\<^sub>c, econf\<^sub>c', R\<^sub>c, G\<^sub>c) \<preceq>\<^sub>e (\<Gamma>\<^sub>a, econf\<^sub>a, R\<^sub>a, G\<^sub>a)) \<or> (
-                    \<exists>econf\<^sub>a' \<delta>\<^sub>a. (\<Gamma>\<^sub>a \<turnstile>\<^sub>a econf\<^sub>a -et-\<delta>\<^sub>a\<rightarrow>econf\<^sub>a') \<and> (gets_e econf\<^sub>a, gets_e econf\<^sub>a') \<in> G\<^sub>a
-                    \<and> (\<Gamma>\<^sub>c, econf\<^sub>c', R\<^sub>c, G\<^sub>c) \<preceq>\<^sub>e (\<Gamma>\<^sub>a, econf\<^sub>a', R\<^sub>a, G\<^sub>a))\<rbrakk> \<Longrightarrow> (\<Gamma>\<^sub>c, econf\<^sub>c, R\<^sub>c, G\<^sub>c) \<preceq>\<^sub>e (\<Gamma>\<^sub>a, econf\<^sub>a, R\<^sub>a, G\<^sub>a)"
+inductive e_sim_validity :: "['Env\<^sub>c, ('l\<^sub>c,'k,'s\<^sub>c,'prog\<^sub>c) econf, ('s\<^sub>c \<times> 's\<^sub>c) set, ('s\<^sub>c \<times> 's\<^sub>c) set, 
+                  ('s\<^sub>c \<times> 's\<^sub>a) set, ('l\<^sub>c,'k,'s\<^sub>c,'prog\<^sub>c) act \<Rightarrow> ('l\<^sub>a,'k,'s\<^sub>a,'prog\<^sub>a) act option, ('s\<^sub>c \<times> 's\<^sub>a) set,
+                  'Env\<^sub>a, ('l\<^sub>a,'k,'s\<^sub>a,'prog\<^sub>a) econf, ('s\<^sub>a \<times> 's\<^sub>a) set, ('s\<^sub>a \<times> 's\<^sub>a) set] \<Rightarrow> bool" 
+  ("'(_,_,_,_')/ \<preceq>\<^sub>e \<^sub>'(\<^sub>_\<^sub>;\<^sub>_\<^sub>;\<^sub>_\<^sub>') /'(_,_,_,_')" [81,81,81,81,81,81,81,81,81,81,81] 100)
+  where rgsim : "\<lbrakk>(s\<^sub>c, s\<^sub>a) \<in> \<alpha>; 
+                  
+                  ((\<Gamma>\<^sub>c \<turnstile>\<^sub>c (e\<^sub>c, s\<^sub>c, x\<^sub>c) -et-(a\<^sub>c\<sharp>k)\<rightarrow> (e\<^sub>c', s\<^sub>c', x\<^sub>c')) \<and> \<zeta> a\<^sub>c = None \<longrightarrow> (s\<^sub>c, s\<^sub>c') \<in> G\<^sub>c \<and>
+                   (\<Gamma>\<^sub>c, (e\<^sub>c', s\<^sub>c', x\<^sub>c'), R\<^sub>c, G\<^sub>c) \<preceq>\<^sub>e \<^sub>(\<^sub>\<alpha>\<^sub>;\<^sub>\<zeta>\<^sub>;\<^sub>\<gamma>\<^sub>) (\<Gamma>\<^sub>a, (e\<^sub>a, s\<^sub>a, x\<^sub>a), R\<^sub>a, G\<^sub>a)) \<and>
 
+                  ((\<Gamma>\<^sub>c \<turnstile>\<^sub>c (e\<^sub>c, s\<^sub>c, x\<^sub>c) -et-(a\<^sub>c\<sharp>k)\<rightarrow> (e\<^sub>c', s\<^sub>c', x\<^sub>c')) \<and> \<zeta> a\<^sub>c = Some a\<^sub>a \<longrightarrow> (\<exists>e\<^sub>a s\<^sub>a x\<^sub>a. 
+                   (\<Gamma>\<^sub>a \<turnstile>\<^sub>a (e\<^sub>a, s\<^sub>a, x\<^sub>a) -et-(a\<^sub>a\<sharp>k)\<rightarrow> (e\<^sub>a', s\<^sub>a', x\<^sub>a')) \<and> (s\<^sub>c, s\<^sub>c') \<in> G\<^sub>c \<and> (s\<^sub>a, s\<^sub>a') \<in> G\<^sub>a \<and> 
+                   (\<Gamma>\<^sub>c, (e\<^sub>c', s\<^sub>c', x\<^sub>c'), R\<^sub>c, G\<^sub>c) \<preceq>\<^sub>e \<^sub>(\<^sub>\<alpha>\<^sub>;\<^sub>\<zeta>\<^sub>;\<^sub>\<gamma>\<^sub>) (\<Gamma>\<^sub>a, (e\<^sub>a', s\<^sub>a', x\<^sub>a'), R\<^sub>a, G\<^sub>a))) \<and>
 
-(*
-inductive pes_sim_validity :: "'Env\<^sub>c \<Rightarrow> ('l\<^sub>c,'k\<^sub>c,'s\<^sub>c,'prog\<^sub>c) pesconf \<Rightarrow> ('s\<^sub>c \<times> 's\<^sub>c) set \<Rightarrow> ('s\<^sub>c \<times> 's\<^sub>c) set
-    \<Rightarrow> 'Env\<^sub>a \<Rightarrow> ('l\<^sub>a,'k\<^sub>a,'s\<^sub>a,'prog\<^sub>a) pesconf \<Rightarrow> ('s\<^sub>a \<times> 's\<^sub>a) set \<Rightarrow> ('s\<^sub>a \<times> 's\<^sub>a) set \<Rightarrow> bool" 
-    ("'(_,_,_,_')/ \<preceq>\<^sub>p\<^sub>e\<^sub>s /'(_,_,_,_')" [81,81,81,81,81,81,81,81] 100)
-    where rgsim : "\<lbrakk>sim_s (gets pesconf\<^sub>c) = gets pesconf\<^sub>a ;
-                    \<forall>pesconf\<^sub>c' \<delta>\<^sub>c. (\<Gamma>\<^sub>c \<turnstile>\<^sub>c pesconf\<^sub>c -pes-\<delta>\<^sub>c\<rightarrow>pesconf\<^sub>c') \<longrightarrow> 
-                    ((\<Gamma>\<^sub>c, pesconf\<^sub>c', R\<^sub>c, G\<^sub>c) \<preceq>\<^sub>p\<^sub>e\<^sub>s (\<Gamma>\<^sub>a, pesconf\<^sub>a, R\<^sub>a, G\<^sub>a)) \<or> (
-                     \<exists>pesconf\<^sub>a' \<delta>\<^sub>a. (\<Gamma>\<^sub>a \<turnstile>\<^sub>a pesconf\<^sub>a -pes-\<delta>\<^sub>a\<rightarrow>pesconf\<^sub>a') \<and> (gets pesconf\<^sub>a, gets pesconf\<^sub>a') \<in> G\<^sub>a
-                     \<and> (\<Gamma>\<^sub>c, pesconf\<^sub>c', R\<^sub>c, G\<^sub>c) \<preceq>\<^sub>p\<^sub>e\<^sub>s (\<Gamma>\<^sub>a, pesconf\<^sub>a', R\<^sub>a, G\<^sub>a)) 
-                    \<rbrakk> \<Longrightarrow> (\<Gamma>\<^sub>c, pesconf\<^sub>c, R\<^sub>c, G\<^sub>c) \<preceq>\<^sub>p\<^sub>e\<^sub>s (\<Gamma>\<^sub>a, pesconf\<^sub>a, R\<^sub>a, G\<^sub>a)"
-*)
+                   (e\<^sub>c = AnonyEvent fin_com\<^sub>c \<longrightarrow> e\<^sub>a = AnonyEvent fin_com\<^sub>a \<and> (s\<^sub>c, s\<^sub>a) \<in> \<gamma>) \<and> 
+
+                   (((s\<^sub>c, s\<^sub>c'), (s\<^sub>a, s\<^sub>a')) \<in> (R\<^sub>c, R\<^sub>a \<union> Id)\<^sub>\<alpha> \<longrightarrow> 
+                     (\<Gamma>\<^sub>c, (e\<^sub>c, s\<^sub>c', x\<^sub>c'), R\<^sub>c, G\<^sub>c) \<preceq>\<^sub>e \<^sub>(\<^sub>\<alpha>\<^sub>;\<^sub>\<zeta>\<^sub>;\<^sub>\<gamma>\<^sub>) (\<Gamma>\<^sub>a, (e\<^sub>a, s\<^sub>a', x\<^sub>a'), R\<^sub>a, G\<^sub>a))      
+                  \<rbrakk> \<Longrightarrow> (\<Gamma>\<^sub>c, (e\<^sub>c, s\<^sub>c, x\<^sub>c), R\<^sub>c, G\<^sub>c) \<preceq>\<^sub>e \<^sub>(\<^sub>\<alpha>\<^sub>;\<^sub>\<zeta>\<^sub>;\<^sub>\<gamma>\<^sub>) (\<Gamma>\<^sub>a, (e\<^sub>a, s\<^sub>a, x\<^sub>a), R\<^sub>a, G\<^sub>a)"
 
 
 
-(*
-definition e_sim_validity :: "'Env\<^sub>c \<Rightarrow> ('l\<^sub>c,'k\<^sub>c,'s\<^sub>c,'prog\<^sub>c) econf \<Rightarrow> ('s\<^sub>c \<times> 's\<^sub>c) set \<Rightarrow> ('s\<^sub>c \<times> 's\<^sub>c) set
-    \<Rightarrow> 'Env\<^sub>a \<Rightarrow> ('l\<^sub>a,'k\<^sub>a,'s\<^sub>a,'prog\<^sub>a) econf \<Rightarrow> ('s\<^sub>a \<times> 's\<^sub>a) set \<Rightarrow> ('s\<^sub>a \<times> 's\<^sub>a) set \<Rightarrow> bool" 
-    ("'(_,_,_,_')/ \<preceq>\<^sub>e /'(_,_,_,_')" [81,81,81,81,81,81,81,81] 100)
-    where "(\<Gamma>\<^sub>c, econf\<^sub>c, R\<^sub>c, G\<^sub>c) \<preceq>\<^sub>e (\<Gamma>\<^sub>a, econf\<^sub>a, R\<^sub>a, G\<^sub>a) \<equiv> True"
-
-definition es_sim_validity :: "'Env\<^sub>c \<Rightarrow> ('l\<^sub>c,'k\<^sub>c,'s\<^sub>c,'prog\<^sub>c) esconf \<Rightarrow> ('s\<^sub>c \<times> 's\<^sub>c) set \<Rightarrow> ('s\<^sub>c \<times> 's\<^sub>c) set
-    \<Rightarrow> 'Env\<^sub>a \<Rightarrow> ('l\<^sub>a,'k\<^sub>a,'s\<^sub>a,'prog\<^sub>a) esconf \<Rightarrow> ('s\<^sub>a \<times> 's\<^sub>a) set \<Rightarrow> ('s\<^sub>a \<times> 's\<^sub>a) set \<Rightarrow> bool" 
-    ("'(_,_,_,_')/ \<preceq>\<^sub>e\<^sub>s /'(_,_,_,_')" [81,81,81,81,81,81,81,81] 100)
-    where "(\<Gamma>\<^sub>c, esconf\<^sub>c, R\<^sub>c, G\<^sub>c) \<preceq>\<^sub>e\<^sub>s (\<Gamma>\<^sub>a, esconf\<^sub>a, R\<^sub>a, G\<^sub>a) \<equiv> True"
-
-definition pes_sim_validity :: "'Env\<^sub>c \<Rightarrow> ('l\<^sub>c,'k\<^sub>c,'s\<^sub>c,'prog\<^sub>c) pesconf \<Rightarrow> ('s\<^sub>c \<times> 's\<^sub>c) set \<Rightarrow> ('s\<^sub>c \<times> 's\<^sub>c) set
-    \<Rightarrow> 'Env\<^sub>a \<Rightarrow> ('l\<^sub>a,'k\<^sub>a,'s\<^sub>a,'prog\<^sub>a) pesconf \<Rightarrow> ('s\<^sub>a \<times> 's\<^sub>a) set \<Rightarrow> ('s\<^sub>a \<times> 's\<^sub>a) set \<Rightarrow> bool" 
-    ("'(_,_,_,_')/ \<preceq>\<^sub>p\<^sub>e\<^sub>s /'(_,_,_,_')" [81,81,81,81,81,81,81,81] 100)
-    where "(\<Gamma>\<^sub>c, pesconf\<^sub>c, R\<^sub>c, G\<^sub>c) \<preceq>\<^sub>p\<^sub>e\<^sub>s (\<Gamma>\<^sub>a, pesconf\<^sub>a, R\<^sub>a, G\<^sub>a) \<equiv> 
-            sim_s (gets pesconf\<^sub>c) = gets pesconf\<^sub>a \<and> 
-            ((pesconf\<^sub>c, pesconf'\<^sub>c) \<in> pesetran \<Gamma>\<^sub>c  \<longrightarrow> (gets pesconf\<^sub>c, gets pesconf'\<^sub>c) \<in> G\<^sub>c \<longrightarrow>
-            ((\<Gamma>\<^sub>c, pesconf\<^sub>c, R\<^sub>c, G\<^sub>c) \<preceq>\<^sub>p\<^sub>e\<^sub>s (\<Gamma>\<^sub>a, pesconf\<^sub>a, R\<^sub>a, G\<^sub>a) \<or> 
-            (pesconf\<^sub>a, pesconf'\<^sub>a) \<in> pestran \<Gamma>\<^sub>a \<and> (gets pesconf\<^sub>a, gets pesconf'\<^sub>a) \<in> G\<^sub>a \<and> 
-            (\<Gamma>\<^sub>c, pesconf'\<^sub>c, R\<^sub>c, G\<^sub>c) \<preceq>\<^sub>p\<^sub>e\<^sub>s (\<Gamma>\<^sub>a, pesconf'\<^sub>a, R\<^sub>a, G\<^sub>a)))"
-*)
 
 
